\documentclass{article}
\usepackage{amsmath}
\usepackage{amssymb}
\usepackage{enumerate}

\title{MAT -- 112: Calculus I and Modeling\\
\large{Solution 3}}
\author{Thomas R. Cameron}
\date{2/16/2018}

\begin{document}
\maketitle

\subsection*{Other Problems}

\paragraph*{Problem 1.}	Here we use the limit definition of the derivative to derive formula for computing the derivative of $x^{2}$, $\sqrt{x}$, and $1/x$. 
\begin{itemize}
\item	Let $f(x)=x^{2}$ and note that
\begin{align*}
\frac{d}{dx}f(x)&=\lim_{h\rightarrow 0}\frac{(x+h)^{2}-x^{2}}{h} \\
&=\lim_{h\rightarrow 0}\frac{[x^{2}+2xh+h^{2}]-[x^{2}]}{h} \\
&=\lim_{h\rightarrow 0}\frac{2xh+h^{2}}{h} \\
&=\lim_{h\rightarrow 0}(2x+h)=2x.
\end{align*}
\item	Let $f(x)=\sqrt{x}$ and note that
\begin{align*}
\frac{d}{dx}f(x)&=\lim_{h\rightarrow 0}\frac{\sqrt{x+h}-\sqrt{x}}{h} \\
&=\lim_{h\rightarrow 0}\frac{\sqrt{x+h}-\sqrt{x}}{h}\left(\frac{\sqrt{x+h}+\sqrt{x}}{\sqrt{x+h}+\sqrt{x}}\right) \\
&=\lim_{h\rightarrow 0}\frac{(x+h)-(x)}{h\left(\sqrt{x+h}+\sqrt{x}\right)} \\
&=\lim_{h\rightarrow 0}\frac{1}{\sqrt{x+h}+\sqrt{x}}=\frac{1}{2\sqrt{x}}.
\end{align*}
\item	Let $f(x)=1/x$ and note that
\begin{align*}
\frac{d}{dx}f(x)&=\lim_{h\rightarrow 0}\frac{\left(\frac{1}{x+h}\right)-\left(\frac{1}{x}\right)}{h} \\
&=\lim_{h\rightarrow 0}\frac{x-(x+h)}{hx(x+h)} \\
&=\lim_{h\rightarrow 0}\frac{-1}{x(x+h)}=-\frac{1}{x^{2}}. 
\end{align*}
\end{itemize}

\end{document}