\documentclass{article}
\usepackage{amsmath}
\usepackage{amsthm}
\usepackage{amssymb}
\usepackage{enumerate}

\makeatletter
\renewcommand{\abstractname}{Instructions}
\makeatother

\title{MAT -- 112: Calculus I and Modeling\\
\large{Product Rule}}
\author{Thomas R. Cameron}
\date{February 12, 2018}

\begin{document}
\maketitle

\begin{abstract}
Write out your own proof of the product using the outline below. Fill in the blanks and follow the prompts given. 
\end{abstract}

\paragraph*{Product Rule.} Let $f$ and $g$ be functions that are differentiable at $x$, then
\[
\frac{d}{dx}(fg)(x)=f^{'}(x)g(x)+f(x)g^{'}(x).
\]
\begin{proof}
Note that
\begin{align*}
\frac{d}{dx}(fg)(x)&=\lim_{h\rightarrow 0}\frac{(fg)(x+h)-fg(x)}{h} \\
&=\lim_{h\rightarrow 0}\frac{f(x+h)g(x+h)-f(x)g(x)}{h} \\
&=\lim_{h\rightarrow 0}\frac{f(x+h)g(x+h) -f(x)g(x+h)+f(x)g(x+h)-f(x)g(x)}{h}\quad\text{(Justify)} \\ 
&=\rule{4cm}{0.15mm}\quad\text{(Use sum limit rule)}\\
&=\lim_{h\rightarrow 0}g(x+h)\lim_{h\rightarrow 0}\frac{f(x+h)-f(x)}{h}+\lim_{h\rightarrow 0}f(x)\lim_{h\rightarrow 0}\frac{g(x+h)-g(x)}{h}\quad\text{(Justify)} \\
&=g(x)f^{'}(x)+f(x)g^{'}(x) \\
&=f^{'}(x)g(x)+f(x)g^{'}(x).
\end{align*}
\end{proof}

\end{document}