\documentclass{article}
\usepackage{amsmath}
\usepackage{amsthm}
\usepackage{amssymb}
\usepackage{enumerate}

\makeatletter
\renewcommand{\abstractname}{Instructions}
\makeatother

\title{MAT -- 112: Calculus I and Modeling\\
\large{Quotient Rule}}
\author{Thomas R. Cameron}
\date{February 14, 2018}

\begin{document}
\maketitle

\begin{abstract}
Write out your own proof of the quotient rule using the outline below. Fill in the blanks and follow the prompts given. 
\end{abstract}

\paragraph*{Quotient Rule.} Let $f$ and $g$ be functions that are differentiable at $x$, where $g(x)\neq 0$, then
\[
\frac{d}{dx}\left(\frac{f}{g}\right)(x)=\frac{f^{'}(x)g(x)-f(x)g^{'}(x)}{[g(x)]^{2}}
\]
\begin{proof}
Note that
\begin{align*}
\frac{d}{dx}\left(\frac{f}{g}\right)(x)&=\lim_{h\rightarrow 0}\frac{\left(\frac{f}{g}\right)(x+h)-\left(\frac{f}{g}\right)(x)}{h} \\
&=\lim_{h\rightarrow 0}\frac{\left(\frac{f(x+h)}{g(x+h)}\right)-\left(\frac{f(x)}{g(x)}\right)}{h} \\
&=\lim_{h\rightarrow 0}\frac{g(x)f(x+h)-f(x)g(x+h)}{h(g(x)g(x+h)}\quad\text{(Justify)} \\
&=\lim_{h\rightarrow 0}\frac{g(x)f(x+h)-g(x)f(x)+g(x)f(x)-f(x)g(x+h)}{hg(x)g(x+h)}\quad\text{(Justify)} \\
&=\rule{4cm}{0.15mm}\quad\text{(Use sum limit rule)}\\
&=\lim_{h\rightarrow 0}g(x)\lim_{h\rightarrow 0}\frac{f(x+h)-f(x)}{hg(x)g(x+h)}-\lim_{h\rightarrow 0}f(x)\lim_{h\rightarrow 0}\frac{g(x+h)-g(x)}{hg(x)g(x+h)}\quad\text{(Justify)} \\
&=\lim_{h\rightarrow 0}\frac{1}{g(x)g(x+h)}\left(g(x)\lim_{h\rightarrow 0}\frac{f(x+h)-f(x)}{h}-f(x)\lim_{h\rightarrow 0}\frac{g(x+h)-g(x)}{h}\right)\quad\text{(Justify)} \\
&=\frac{1}{[g(x)]^{2}}\left(g(x)f^{'}(x)-f(x)g^{'}(x)\right) \\
&=\frac{f^{'}(x)g(x)-f(x)g^{'}(x)}{[g(x)]^{2}}.
\end{align*}
\end{proof}

\end{document}